misc/queue-basic-known.bpl
@@ -1,0 +1,350 @@
+// ----------------------------------------
+// A simple queue implementation
+// based on the Michael-Scott queue.
+// Assumes GC, so does not free dequeued nodes.
+// Also uses the simplified heap encoding from CIVL's Treiber example.
+//
+// Use options -noinfer -typeEncoding:m -useArrayTheory
+// ----------------------------------------
+
+type Loc;
+const null: Loc;
+
+type Heap;
+function {:linear "Node"} dom(Heap): [Loc]bool;
+function next(Heap): [Loc]Loc;
+function {:builtin "MapConst"} MapConstBool(bool) : [Loc]bool;
+
+function EmptyHeap(): (Heap);
+axiom (dom(EmptyHeap()) == MapConstBool(false));
+
+function Add(h: Heap, l: Loc, v: Loc): (Heap);
+axiom (forall h: Heap, l: Loc, v: Loc :: dom(Add(h, l, v)) == dom(h)[l:=true] && next(Add(h, l, v)) == next(h)[l := v]);
+
+function Remove(h: Heap, l: Loc): (Heap);
+axiom (forall h: Heap, l: Loc :: dom(Remove(h, l)) == dom(h)[l:=false] && next(Remove(h, l)) == next(h));
+
+// Linearity stuff:
+
+function {:inline} {:linear "Node"} NodeSetCollector(x: [Loc]bool) : [Loc]bool
+{
+  x
+}
+
+
+// ---------- Reachability, between, and associated theories
+
+function Equal([Loc]bool, [Loc]bool) returns (bool);
+function Subset([Loc]bool, [Loc]bool) returns (bool);
+
+function Empty() returns ([Loc]bool);
+function Singleton(Loc) returns ([Loc]bool);
+function Union([Loc]bool, [Loc]bool) returns ([Loc]bool);
+
+axiom(forall x:Loc :: !Empty()[x]);
+
+axiom(forall x:Loc, y:Loc :: {Singleton(y)[x]} Singleton(y)[x] <==> x == y);
+axiom(forall y:Loc :: {Singleton(y)} Singleton(y)[y]);
+
+axiom(forall x:Loc, S:[Loc]bool, T:[Loc]bool :: {Union(S,T)[x]}{Union(S,T),S[x]}{Union(S,T),T[x]} Union(S,T)[x] <==> S[x] || T[x]);
+
+axiom(forall S:[Loc]bool, T:[Loc]bool :: {Equal(S,T)} Equal(S,T) <==> Subset(S,T) && Subset(T,S));
+axiom(forall x:Loc, S:[Loc]bool, T:[Loc]bool :: {S[x],Subset(S,T)}{T[x],Subset(S,T)} S[x] && Subset(S,T) ==> T[x]);
+axiom(forall S:[Loc]bool, T:[Loc]bool :: {Subset(S,T)} Subset(S,T) || (exists x:Loc :: known(x) && S[x] && !T[x]));
+
+
+// Predicates used to control the triggers on the below axioms
+function known(x: Loc) : bool;
+function knownF(f: [Loc]Loc) : bool;
+axiom(forall x: Loc :: {known(x)} known(x));
+axiom(forall f: [Loc]Loc :: {knownF(f)} knownF(f));
+
+ 
+////////////////////
+// Between predicate
+////////////////////
+function Between(f: [Loc]Loc, x: Loc, y: Loc, z: Loc) returns (bool);
+function Avoiding(f: [Loc]Loc, x: Loc, y: Loc, z: Loc) returns (bool);
+
+
+//////////////////////////
+// Between set constructor
+//////////////////////////
+function BetweenSet(f: [Loc]Loc, x: Loc, z: Loc) returns ([Loc]bool);
+
+////////////////////////////////////////////////////
+// axioms relating Between and BetweenSet
+////////////////////////////////////////////////////
+axiom(forall f: [Loc]Loc, x: Loc, y: Loc, z: Loc :: {BetweenSet(f, x, z)[y]} BetweenSet(f, x, z)[y] <==> Between(f, x, y, z));
+axiom(forall f: [Loc]Loc, x: Loc, y: Loc, z: Loc :: {Between(f, x, y, z), BetweenSet(f, x, z)} Between(f, x, y, z) ==> BetweenSet(f, x, z)[y]);
+axiom(forall f: [Loc]Loc, x: Loc, z: Loc :: {BetweenSet(f, x, z)} Between(f, x, x, x));
+axiom(forall f: [Loc]Loc, x: Loc, z: Loc :: {BetweenSet(f, x, z)} Between(f, z, z, z));
+
+
+//////////////////////////
+// Axioms for Between
+//////////////////////////
+
+// read null
+axiom (forall f: [Loc]Loc :: f[null] == null);
+
+// reflexive
+axiom(forall f: [Loc]Loc, x: Loc :: Between(f, x, x, x));
+
+// step
+axiom(forall f: [Loc]Loc, x: Loc :: {f[x]} Between(f, x, f[x], f[x]));
+
+// reach
+axiom(forall f: [Loc]Loc, x: Loc, y: Loc :: {f[x], known(y)} Between(f, x, y, y) ==> x == y || Between(f, x, f[x], y));
+
+// cycle
+axiom(forall f: [Loc]Loc, x: Loc, y:Loc :: {f[x], known(y)} f[x] == x && Between(f, x, y, y) ==> x == y);
+
+// sandwich
+axiom(forall f: [Loc]Loc, x: Loc, y: Loc :: {knownF(f), known(x), known(y), Between(f, x, y, x)} Between(f, x, y, x) ==> x == y);
+
+// order1
+axiom(forall f: [Loc]Loc, x: Loc, y: Loc, z: Loc :: {knownF(f), known(x), known(y), known(z), Between(f, x, y, y), Between(f, x, z, z)} Between(f, x, y, y) && Between(f, x, z, z) ==> Between(f, x, y, z) || Between(f, x, z, y));
+
+// order2
+axiom(forall f: [Loc]Loc, x: Loc, y: Loc, z: Loc :: {knownF(f), known(x), known(y), known(z), Between(f, x, y, z)} Between(f, x, y, z) ==> Between(f, x, y, y) && Between(f, y, z, z));
+
+// transitive1
+axiom(forall f: [Loc]Loc, x: Loc, y: Loc, z: Loc :: {knownF(f), known(x), known(y), known(z), Between(f, x, y, y), Between(f, y, z, z)} Between(f, x, y, y) && Between(f, y, z, z) ==> Between(f, x, z, z));
+
+// transitive2
+axiom(forall f: [Loc]Loc, x: Loc, y: Loc, z: Loc, w: Loc :: {knownF(f), known(x), known(y), known(z), known(w), Between(f, x, y, z), Between(f, y, w, z)} Between(f, x, y, z) && Between(f, y, w, z) ==> Between(f, x, y, w) && Between(f, x, w, z));
+
+// transitive3
+axiom(forall f: [Loc]Loc, x: Loc, y: Loc, z: Loc, w: Loc :: {knownF(f), known(x), known(y), known(z), known(w), Between(f, x, y, z), Between(f, x, w, y)} Between(f, x, y, z) && Between(f, x, w, y) ==> Between(f, x, w, z) && Between(f, w, y, z));
+
+// relation between Avoiding and Between
+axiom(forall f: [Loc]Loc, x: Loc, y: Loc, z: Loc :: {knownF(f), known(x), known(y), known(z), Avoiding(f, x, y, z)} Avoiding(f, x, y, z) <==> (Between(f, x, y, z) || (Between(f, x, y, y) && !Between(f, x, z, z))));
+axiom(forall f: [Loc]Loc, x: Loc, y: Loc, z: Loc :: {knownF(f), known(x), known(y), known(z), Between(f, x, y, z)} Between(f, x, y, z) <==> (Avoiding(f, x, y, z) && Avoiding(f, x, z, z)));
+
+// btwn_write: grasshopper's update axiom
+axiom (forall f: [Loc]Loc, x: Loc, y: Loc, z: Loc, u: Loc, v: Loc :: {f[u := v], known(x), known(y), known(z), Between(f[u := v], x, y, z)}
+        u != null ==>
+          (Between(f[u := v], x, y, z) <==>
+          (Between(f, x, y, z) && Avoiding(f, x, z, u))
+          || (u != z && Avoiding(f, x, u, z) && Avoiding(f, v, z, u)
+            && (Between(f, x, y, u) || Between(f, v, y, z)))));
+
+
+// ---------- Shared state and invariant
+
+var {:linear "Node"} {:layer 0,2} queue: Heap;
+var {:linear "Node"} {:layer 0,2} Used: [Loc]bool;
+
+var {:layer 0,2} head: Loc;
+var {:layer 0,2} tail: Loc;
+
+
+function {:inline} Inv(queue: Heap, head: Loc, tail: Loc) : (bool)
+{
+  Between(next(queue), head, head, null)
+    && Between(next(queue), head, tail, null)
+    && Equal(BetweenSet(next(queue), head, null),
+             Union(Singleton(null), dom(queue)))
+    && tail != null
+    && known(head) && known(tail) && known(null) && knownF(next(queue))
+}
+
+
+// ---------- Primitives for manipulating ghost state
+
+procedure {:atomic} {:layer 1} AtomicReadhead() returns (v:Loc)
+{ v := head; }
+
+procedure {:yields} {:layer 0} {:refines "AtomicReadhead"} Readhead() returns (v:Loc);
+
+procedure {:atomic} {:layer 1} AtomicReadtail() returns (v:Loc)
+{ v := tail; }
+
+procedure {:yields} {:layer 0} {:refines "AtomicReadtail"} Readtail() returns (v:Loc);
+
+procedure {:atomic} {:layer 1} AtomicLoad(i:Loc) returns (v:Loc)
+{
+  assert dom(queue)[i] || Used[i];
+  if (dom(queue)[i]) {
+    v := next(queue)[i];
+    assume known(v);
+  }
+}
+
+procedure {:yields} {:layer 0} {:refines "AtomicLoad"} Load(i:Loc) returns (v:Loc);
+
+procedure {:both} {:layer 1} AtomicStore({:linear_in "Node"} l_in:Heap, i:Loc, v:Loc) returns ({:linear "Node"} l_out:Heap)
+{ assert dom(l_in)[i]; l_out := Add(l_in, i, v); assume knownF(next(l_in)); }
+
+procedure {:yields} {:layer 0} {:refines "AtomicStore"} Store({:linear_in "Node"} l_in:Heap, i:Loc, v:Loc) returns ({:linear "Node"} l_out:Heap);
+
+
+procedure {:atomic} {:layer 1} AtomicTransferToqueue(t: Loc, oldVal: Loc,
+    newVal: Loc, {:linear_in "Node"} l_in:Heap)
+  returns (r: bool, {:linear "Node"} l_out:Heap)
+  modifies queue;
+{
+  assert dom(l_in)[newVal];
+  if (next(queue)[t] == oldVal) {
+    queue := Add(queue, t, newVal);
+    l_out := EmptyHeap();
+    queue := Add(queue, newVal, next(l_in)[newVal]);
+    assume known(oldVal) && known(newVal) && known(next(l_in)[newVal]) && knownF(next(queue));
+    r := true;
+  } else {
+    l_out := l_in;
+    r := false;
+  }
+}
+
+procedure {:yields} {:layer 0} {:refines "AtomicTransferToqueue"}
+  TransferToqueue(t: Loc, oldVal: Loc, newVal: Loc,
+                  {:linear_in "Node"} l_in:Heap)
+  returns (r: bool, {:linear "Node"} l_out:Heap);
+
+procedure {:atomic} {:layer 1} AtomicTransferFromqueue(oldVal: Loc, newVal: Loc) returns (r: bool)
+  modifies head, Used, queue;
+{
+  if (oldVal == head) {
+    head := newVal;
+    Used[oldVal] := true;
+    queue := Remove(queue, oldVal);
+    assume known(oldVal) && known(head) && knownF(next(queue));
+    r := true;
+  }
+  else {
+    r := false;
+  }
+}
+
+procedure {:yields} {:layer 0} {:refines "AtomicTransferFromqueue"} TransferFromqueue(oldVal: Loc, newVal: Loc) returns (r: bool);
+
+
+// ---------- queue methods:
+
+procedure {:atomic} {:layer 2} atomic_pop() returns (t: Loc)
+  modifies Used, head, queue;
+{
+  assume head != null;
+  t := head;
+  Used[t] := true;
+  head := next(queue)[t];
+  queue := Remove(queue, t);
+  assume known(head) && knownF(next(queue));
+}
+
+procedure {:yields} {:layer 1} {:refines "atomic_pop"} pop() returns (h: Loc)
+requires {:layer 1} Inv(queue, head, tail);
+ensures {:layer 1} Inv(queue, head, tail);
+{
+  var g: bool;
+  var t, x: Loc;
+
+  yield;
+  assert {:layer 1} Inv(queue, head, tail);
+  while (true)
+    invariant {:layer 1} Inv(queue, head, tail);
+  {
+    call h := Readhead();
+    yield;
+    assert {:layer 1} Inv(queue, head, tail);
+    assert {:layer 1} h == head || Used[h];
+
+    call t := Readtail();
+    yield;
+    assert {:layer 1} Inv(queue, head, tail);
+    assert {:layer 1} h == head || Used[h];
+    assert {:layer 1} (h == head && h != t ==> head != tail);
+
+    if (h != t) {
+      call x := Load(h);
+      yield;
+      assert {:layer 1} Inv(queue, head, tail);
+      assert {:layer 1} h == head || Used[h];
+      assert {:layer 1} (h == head && h != t ==> x == next(queue)[head]);
+      assert {:layer 1} (h == head && h != t ==> head != tail);
+
+      call g := TransferFromqueue(h, x);
+      if (g) {
+        break;
+      }
+    }
+    yield;
+    assert {:layer 1} Inv(queue, head, tail);
+  }
+  yield;
+  assert {:expand} {:layer 1} Inv(queue, head, tail);
+}
+
+
+procedure {:atomic} {:layer 2} atomic_push(x: Loc,
+ {:linear_in "Node"} x_Heap: Heap)
+ modifies queue, tail;
+{
+  if (next(queue)[tail] == null) {
+    queue := Add(queue, tail, x);
+    queue := Add(queue, x, null);
+  }
+  // tail := x;
+}
+
+procedure {:yields} {:layer 1} {:refines "atomic_push"} push(x: Loc, {:linear_in "Node"} x_Heap: Heap)
+  requires {:layer 1} dom(x_Heap)[x] && next(x_Heap)[x] == null;
+  requires {:layer 1} Inv(queue, head, tail);
+  ensures {:layer 1} Inv(queue, head, tail);
+{
+  var t, tn: Loc;
+  var g: bool;
+  var {:linear "Node"} t_Heap: Heap;
+
+  yield;
+  assert {:layer 1} Inv(queue, head, tail);
+  assert {:layer 1} known(t) && known(tn);
+  t_Heap := x_Heap;
+  while (true)
+    invariant {:layer 1} dom(t_Heap) == dom(x_Heap);
+    invariant {:layer 1} next(t_Heap)[x] == null; // TODO needed?
+    invariant {:layer 1} Inv(queue, head, tail);
+    invariant {:layer 1} known(t) && known(tn);
+  {
+    call t := Readtail();
+    yield;
+    assert {:layer 1} Inv(queue, head, tail);
+    assert {:layer 1} known(t) && known(tn);
+    assert {:layer 1} dom(t_Heap) == dom(x_Heap);
+    assert {:layer 1} next(t_Heap)[x] == null;
+    assert {:layer 1} t != null && (Between(next(queue), head, t, null)
+      || Used[t]);
+    assert {:layer 1} next(queue)[t] == null ==> t == tail;
+
+    call tn := Load(t);
+    yield;
+    assert {:layer 1} Inv(queue, head, tail);
+    assert {:layer 1} known(t) && known(tn);
+    assert {:layer 1} dom(t_Heap) == dom(x_Heap);
+    assert {:layer 1} next(t_Heap)[x] == null;
+    assert {:layer 1} t != null && (Between(next(queue), head, t, null)
+      || Used[t]);
+    assert {:layer 1} next(queue)[t] == null ==> t == tail;
+
+    if (tn == null) {
+      call g, t_Heap := TransferToqueue(t, tn, x, t_Heap);
+      if (g) {
+        break;
+      }
+    } // TODO else cas tail
+    yield;
+    assert {:layer 1} dom(t_Heap) == dom(x_Heap);
+    assert {:layer 1} Inv(queue, head, tail);
+    assert {:layer 1} known(t) && known(tn);
+  }
+  yield;
+  assert {:layer 1} known(head) && known(tail) && known(null) && knownF(next(queue));
+  assert {:layer 1} Between(next(queue), head, head, null);
+  assert {:layer 1} Between(next(queue), head, tail, null);
+  assert {:layer 1} Equal(BetweenSet(next(queue), head, null),
+             Union(Singleton(null), dom(queue)));
+  assert {:layer 1} tail != null;
+  assert {:expand} {:layer 1} Inv(queue, head, tail);
+}
